### Program Locality Homework

<center>Jiupeng Zhang</center>





1. **Consider the abc examples in Figure 1. Give the order that has the best locality and show that the order is indeed optimal.** 

   **Answer:** The order with the best locality and its corresponding *reuse distances* are:

   $\begin{matrix}\space rd:\space\space\space\space\space\space \infty&1&\infty&1&\infty&1 \\trace:\space\space a&a&b&b&c&c \end{matrix} $



   The *miss ratio* when $c = 1$ for the above sequence is: 

   $mr(1) = P(rd > 1) =  \frac{3}{6} = 0.5$.



   Assume there exists an order with a miss ratio less than 0.5, in other words, we must have less than 3 misses during the access. However, apparently, this is not possible because 3 misses must happen in this example ($m = 3$) when we first visit *a*, *b* and *c*.

   That is to say, for any cache with size $c \ge 1$ in this example, the miss ratio $mr(c) \ge 0.5 $ , so "a a b b c c" is an optimal order with the best locality.



2. - **Prove that in the limit form Xiang formula, we always have fp(0) = 0.**

     **Answer:** The limit form Xiang formula is:

     $\lim_{n \to \infty}fp(x) = m -  \sum_{i=x + 1}^{\infty}{(i - x)P(rt = i)} $

     For $x = 0$, $\lim_{n \to \infty}fp(0) = m -  \sum_{i=1}^{\infty}{iP(rt = i)} $ ***— Eq. 1***



     Now, consider the infinite long $n = \infty$ trace has a cycle $C$ with a size of $c$, indicates that all data blocks will be visited in a single loop, such that the size of distinct data blocks  $m$ within the whole trace is the same as the $m$ in $C$.



     The ***Eq. 1*** defined $P(rt=i)$ as the portion of accesses that have reuse time *i*, thus

     $\sum_{i = 1}^{\infty}iP(rt = i) = \sum_{i = 1}^{\infty}i\frac{rt(i)} c$ ***— Eq. 2***



     As we can see, *c* equals to the number of accesses in within a cycle.

     Then, we define $B^j (j \in [1, m])$ as the $j_{th}$ distinct data block in a cycle, so $rt(B^j, i)$ represents the number of accesses on the $j_{th}$ block whose reuse time is *i*, therefore

     $\sum_{i = 1}^{\infty}iP(rt = i) = \sum_{j=1}^{m}\sum_{i = 1}^{\infty}i\frac{rt(B^j, i)} c$ ***— Eq. 3***



     Combined ***Eq. 3*** with ***Eq. 1***, so that

     $\lim_{n \to \infty}fp(0) = m - \sum_{j=1}^{m}\sum_{i = 1}^{\infty}i\frac{rt(B^j, i)} c $ ***— Eq. 4***



     For each distinct data block $B$, we know that $\sum_{i=1}^{\infty}i \times rt(B, i) = c$, substituting is into ***Eq. 4***, we get

     $\lim_{n \to \infty}fp(0) = m - \frac{m\times c} {c} = m - m = 0 $



     Therefore, $fp(0) = 0$.




   - **Does the conclusion hold for finite length traces? If yes, give a proof; otherwise, show a counter example.**

     **Answer:** The Xiang formula is:

     $\lim_{n \to \infty}fp(x) = m -  \frac{1} {n - x + 1}\Big(\sum_{i=x + 1}^{n - 1}{(i - x)rt(i) + \sum_{k=1}^{m}(f_k - x)I(f_k \gt x) + \sum_{k=1}^{m}(l_k - x)I(l_k \gt x)}\Big) $

     For $x = 0$, $\lim_{n \to \infty}fp(0) = m -  \frac{1} {n + 1}\Big(\sum_{i=1}^{n - 1}{i\times rt(i) + \sum_{k=1}^{m}f_k \times I(f_k \gt 0) + \sum_{k=1}^{m}l_k\times I(l_k \gt 0)}\Big)$



     Since $\sum_{k=1}^{m}f_k \times I(f_k \gt 0) + \sum_{k=1}^{m}l_k\times I(l_k \gt 0) = \sum_{k=1}^{m}(f_k + l_k + rt_k - rt_k\Big)$, so

     $\lim_{n \to \infty}fp(0) = m -  \frac{1} {n + 1}\Big(\sum_{i=1}^{n - 1}{i\times rt(i) + \sum_{k=1}^{m}(f_k + l_k + rt_k - rt_k\Big)}$



     For $f_k + l_k + rt_k = n  + 1$, we can derive

     $\lim_{n \to \infty}fp(0) = m -  \frac{1} {n + 1}\Big(\sum_{i=1}^{n - 1}{i\times rt(i) + m(n + 1) - \sum_{k=1}^{m}rt_k\Big)}$



     Besides, as two representatives of total reuse distance in the trace, $\sum_{i=1}^{n-1}i\times rt(i) = \sum_{k=1}^{m}rt_k$, so that

     $\lim_{n \to \infty}fp(0) = m -  \frac{1} {n + 1} {\Big(m(n + 1)\Big)} = m - m = 0$



     Therefore, for finite length traces, $fp(0) = 0$.

3. - **Show the derivation from P (A, rt = i) in Figure 3 to fp(A, x) in Figure 4.**

     **Answer:** Reference from the reuse time distributions in *Figure 3*:

     | i    | $P(A, rt=i)$ | $P(B, rt=i)$ | $P(rt=i)$ |
     | ---- | ------------ | ------------ | --------- |
     | *1*  | 1/3          | 0            | 1/3       |
     | *2*  | 1/3          | 0            | 1/3       |
     | *3M* | 0            | 1/3          | 1/3       |

     $fp(A,0) = 1 - \Big(P(A, rt=1) + 2 \times P(A, rt=2)\Big) = 1 - \Big(\frac 1 3 + 2 \times \frac 1 3\Big) = 0$

     $fp(A,1) = 1 - P(A, rt=2) = 1 - \frac 1 3 = \frac 2 3$

     $fp(A,2) = fp(A,3 \le x \lt 3M) = fp(A,x \ge 3M) = 1 - 0 = 1$




   - **Show the derivation from fp(B, x) to the miss ratio of array B in its single-array cache mrB(c) and the two-array cache mrAB(B,c).**



     $mr_B(0) = fp(B, 1) - fp(B, 0) = \frac 1 3 - 0 =\frac 1 3 $

     $mr_B(\frac 1 3) = fp(B, 2) - fp(B, 1) = \frac 2 3 - \frac 1 3 = \frac 1 3$

     $mr_B(c \lt M) = fp(B, x + 1) -  fp(B, x) |_{fp(B, x) = c}= \frac {x + 1} 3 - \frac x 3 = \frac 1 3$

     $mr_B(c \ge M) =  fp(B, x + 1) -  fp(B, x) |_{fp(B, x) = c}= M - M = 0$



     $mr_{AB}(B, 0) = fp(B, 1) - fp(B, 0) = \frac 1 3 - 0 =\frac 1 3$

     $mr_{AB}(B, 1) = fp(B, 2) - fp(B, 1) = \frac 2 3 - \frac 1 3 = \frac 1 3$

     $mr_{AB}(B, \frac 5 3) =  fp(B, 3) - fp(B, 2) = \frac 3 3 - \frac 2 3 = \frac 1 3$

     $mr_{AB}(B, c \le M) = fp(B, x + 1) -  fp(B, x) |_{fp(x) = c}= \frac {x + 1} 3 - \frac x 3 = \frac 1 3$

     $mr_{AB}(B, c \gt M) = fp(B, x + 1) -  fp(B, x) |_{fp(x) = c}= M - M = 0$


